Steel impl of low-level vget/vput

steel/Veritas.Steel.Verifier.fsti
@@ -1,263 +1,118 @@
 module Veritas.Steel.Verifier
 
-open FStar.Ghost
 open Steel.Memory
 open Steel.Effect.Atomic
 open Steel.Effect
 open Steel.Reference
 open Steel.Array
+open FStar.Ghost
 module U32 = FStar.UInt32
 module U64 = FStar.UInt64
 
-module K = Veritas.Key
-module R = Veritas.Record
-module L = Veritas.Intermediate.Logs
-module S = Veritas.Intermediate.Store
-module V = Veritas.Intermediate.Verify
-module VC = Veritas.Intermediate.VerifierConfig
-module MS = Veritas.MultiSetHashDomain
-
 module T = Veritas.Formats.Types
 
-#set-options "--ide_id_info_off"
+open Veritas.Steel.VCache
+open Veritas.Steel.VerifierModel
 
-#push-options "--fuel 0 --ifuel 0"
-
-(** Definition of the low-level thread state datatype **)
-
-let data_key_t = T.key
-let data_value_t = T.data_value
-
-// AF: Some assumed correspondance between low-level and intermediate types
-val key_v (k:data_key_t) : K.data_key
-val value_v (v:data_value_t) : R.data_value
-
-(* Low-level definition of slot_id *)
-let slot_t (vcfg:VC.verifier_config) = (i:U32.t{U32.v i < VC.store_size vcfg})
-
-// AF: Temporary placeholder for low-level clock.
-// Should be replaced by the appropriate low-level type
-let timestamp_t = ref MS.timestamp
-
-// AF: Placeholder for low-level version of the thread local store
-let vstore_t (vcfg:VC.verifier_config) = array (option T.record)
-
-val to_vstore_entry (vcfg:VC.verifier_config) (r:T.record) : S.vstore_entry vcfg
-
-// AF: This will be implemented as an array.
-// But it also needs to encapsulate the invariants to provide a selector to store
-// instead of store_raw
-// A simple way would be to add those as pure predicates in the slprop, but
-// an easier mechanism for selector invariants/refinements would be useful
-val vstore_sl (#vcfg:_) (st:vstore_t vcfg) : slprop u#1
-val vstore_sel (#vcfg:_) (st:vstore_t vcfg) : selector (S.vstore vcfg) (vstore_sl st)
-
-[@@__steel_reduce__]
-let is_vstore' #vcfg (st:vstore_t vcfg) : vprop' =
-  { hp = vstore_sl st;
-    t = S.vstore vcfg;
-    sel = vstore_sel st }
-unfold
-let is_vstore #vcfg (st:vstore_t vcfg) : vprop = VUnit (is_vstore' st)
-
-[@@ __steel_reduce__]
-let v_st (#p:vprop) (#vcfg:_) (st:vstore_t vcfg)
-  (h:rmem p{FStar.Tactics.with_tactic selector_tactic (can_be_split p (is_vstore st) /\ True)})
-  : GTot (S.vstore vcfg)
-  = h (is_vstore st)
-
-let option_map (#a #b:Type) (f:a -> b) (x:option a) : option b = match x with
-  | None -> None
-  | Some v -> Some (f v)
-
-let vstore_get_record (#vcfg:_) (st:vstore_t vcfg) (s:slot_t vcfg)
-  : Steel
-      (option T.record) // (S.vstore_entry vcfg))
-      (is_vstore st)
-      (fun _ -> is_vstore st)
-      (requires fun h -> True)
-      (ensures fun h0 res h1 ->
-        // Framing
-        v_st st h0 == v_st st h1 /\
-        // Functional correctness
-        (None? res <==> None? (S.get_slot (v_st st h1) (U32.v s)))
-        // res == (Seq.index (v_st st h1) (U32.v s))
-      )
-  =
-  // All the proof steps should disappear once we define is_vstore as a varray of max_length U32
-  rewrite_slprop (is_vstore st) (varray st) (fun _ -> admit());
-  let h = get () in
-  assume (U32.v s < length (asel st h));
-  let res = index st s in
-  rewrite_slprop (varray st) (is_vstore st) (fun _ -> admit());
-  admit();
-  return res
-
-let vstore_update_record (#vcfg:_) (st:vstore_t vcfg) (s:slot_t vcfg) (r:data_value_t)
-  : Steel unit
-      (is_vstore st)
-      (fun _ -> is_vstore st)
-      (requires fun h0 -> True)
-        // S.inuse_slot (v_st st h0) (U32.v s) /\
-        // K.is_data_key (S.stored_key (v_st st h0) (U32.v s)))
-      (ensures fun h0 _ h1 -> True)
-        // S.inuse_slot (v_st st h0) (U32.v s) /\
-        // K.is_data_key (S.stored_key (v_st st h0) (U32.v s))
-        // Functional correctness
-//        v_st st h1 == S.update_value (v_st st h0) (U32.v s) (R.DVal (value_v r)))
-  = rewrite_slprop (is_vstore st) (varray st) (fun _ -> admit());
-  let h = get () in
-  assume (U32.v s < length (asel st h));
-  let r0 = index st s in
-  (match r0 with
-  | None ->
-    // This should be a failure
-     noop (); ()
-  | Some r0 ->
-    let r = {r0 with T.record_value = T.V_dval r} in
-    noop ();
-    upd st s (Some r));
-  rewrite_slprop (varray st) (is_vstore st) (fun _ -> admit())
-
-
-// AF: Placeholder for the low-level version of the multiset hash
 val prf_set_hash : Type0
+
 // AF: Internally, should probably be implemented with a ghost reference to the model_hash
 // The selector would then fetch the value in the ghost state
 // The reason why we would need a ghost state is that the "spec" contains strictly more
 // information than the concrete value. So we cannot reconstruct it out of just the concrete state
 val prf_set_hash_sl (_:prf_set_hash) : slprop u#1
-val prf_set_hash_sel (r:prf_set_hash) : selector MS.ms_hash_value (prf_set_hash_sl r)
+val prf_set_hash_sel (r:prf_set_hash) : selector (model_hash) (prf_set_hash_sl r)
 [@@__steel_reduce__]
 let prf_set_hash_inv' (r:prf_set_hash) : vprop' =
   { hp = prf_set_hash_sl r;
-    t = MS.ms_hash_value;
+    t = model_hash;
     sel = prf_set_hash_sel r}
 unfold
 let prf_set_hash_inv (r:prf_set_hash) : vprop = VUnit (prf_set_hash_inv' r)
 
-(* Standard Steel helper to access the selector of the hash without repeating the slprop *)
 [@@ __steel_reduce__]
 let v_hash (#p:vprop) (r:prf_set_hash)
   (h:rmem p{FStar.Tactics.with_tactic selector_tactic (can_be_split p (prf_set_hash_inv r) /\ True)})
-  : GTot MS.ms_hash_value
+  : GTot model_hash
   = h (prf_set_hash_inv r)
 
-(* Low-level struct representing the current state of a thread *)
+let thread_id = U32.t
+let counter_t = ref U64.t
+
 noeq
-type thread_state_t vcfg = {
-  failed       : ref bool;
-  id           : L.thread_id;
-  st           : vstore_t vcfg;  //a map from keys (cache ids) to merkle leaf or internal nodes
-  clock        : timestamp_t;
+type thread_state_t = {
+  id           : thread_id;
+  st           : vstore;  //a map from keys (cache ids) to merkle leaf or internal nodes
+  clock        : counter_t;
   hadd         : prf_set_hash; //current incremental set hash values; TODO
   hevict       : prf_set_hash;
+  failed       : ref bool
 }
 
-(* The separation logic assertion representing the validity of the thread state *)
 [@@__reduce__; __steel_reduce__]
-let thread_state_inv #vcfg (t:thread_state_t vcfg) : vprop =
+let thread_state_inv (t:thread_state_t) : vprop =
   is_vstore t.st `star`
   vptr t.clock `star`
   vptr t.failed `star`
   prf_set_hash_inv t.hadd `star`
   prf_set_hash_inv t.hevict
 
-let do_vtls (#vcfg:_) (valid:bool)
-  (id:L.thread_id)
-  (st:S.vstore vcfg)
-  (clock:MS.timestamp)
-  (hadd hevict:MS.ms_hash_value) : V.vtls vcfg
-  = if valid then V.Valid id st clock hadd hevict else V.Failed
-
-(* An abstraction on top of the thread selector state to match with the intermediate
-   thread state representation *)
 [@@ __steel_reduce__]
 unfold
-let v_thread (#p:vprop) (#vcfg:_) (t:thread_state_t vcfg)
+let v_thread (#p:vprop) (t:thread_state_t)
   (h:rmem p{FStar.Tactics.with_tactic selector_tactic (can_be_split p (thread_state_inv t) /\ True)})
-  : GTot (V.vtls vcfg)
-  = let valid = sel t.failed (focus_rmem h (thread_state_inv t)) in
-    let st = v_st t.st (focus_rmem h (thread_state_inv t)) in
-    let clock = sel t.clock (focus_rmem h (thread_state_inv t)) in
-    let hadd = v_hash t.hadd (focus_rmem h (thread_state_inv t)) in
-    let hevict = v_hash t.hevict (focus_rmem h (thread_state_inv t)) in
-    do_vtls valid t.id st clock hadd hevict
+  : GTot thread_state_model
+  = {
+      model_failed = sel t.failed (focus_rmem h (thread_state_inv t));
+      model_store = asel t.st (focus_rmem h (thread_state_inv t));
+      model_clock = sel t.clock (focus_rmem h (thread_state_inv t));
+      model_hadd = v_hash t.hadd (focus_rmem h (thread_state_inv t));
+      model_hevict = v_hash t.hevict (focus_rmem h (thread_state_inv t))
+    }
 
-(* Updates the thread state to a Failed state *)
-let fail #vcfg (vs:thread_state_t vcfg) (msg:string)
-  // AF: We put it in SteelF to avoid simplify its use in branches because we currently
-  // cannot have Steel and SteelF branches at the same time, but it shouldn't be
+let fail (vs:thread_state_t) (msg:string)
   : SteelF unit
              (thread_state_inv vs)
              (fun _ -> thread_state_inv vs)
              (requires fun _ -> True)
-             (ensures fun _ _ h1 -> v_thread vs h1 == V.Failed)
-  = // AF: Need trailing unit to trigger framing. Will be solved once we have framing subcomp
-    write vs.failed false;
-    ()
+             (ensures fun h0 _ h1 -> v_thread vs h1 == model_fail (v_thread vs h0))
+  = write vs.failed false; ()
 
-#push-options "--ifuel 1 --z3rlimit 20"
+#push-options "--fuel 0 --ifuel 0"
 
-(* An implementation of Veritas.Intermediate.Verify.vget *)
-let vget (#vcfg:_) (s:slot_t vcfg) (k:data_key_t) (v:data_value_t) (vs:thread_state_t vcfg)
+let vget (s:U32.t) (v:T.value) (vs: thread_state_t)
   : Steel unit
-             (thread_state_inv vs)
-             (fun _ -> thread_state_inv vs)
-             (requires fun h0 ->
-               V.Valid? (v_thread vs h0))
-             (ensures fun h0 _ h1 ->
-               V.Valid? (v_thread vs h0) /\
-               v_thread vs h1 == V.vget (U32.v s) (key_v k) (value_v v) (v_thread vs h0)
-             )
-  = let h = get () in
-    // assert (V.Valid? (v_thread vs h));
-    assert (v_st vs.st h == V.thread_store (v_thread vs h));
-
-
-    let r0 = vstore_get_record vs.st s in
-
-
-    match r0 with
+          (thread_state_inv vs)
+          (fun _ -> thread_state_inv vs)
+          (requires fun h -> U32.v s < length (v_thread vs h).model_store)
+          (ensures fun h0 _ h1 ->
+            U32.v s < length (v_thread vs h0).model_store /\
+            v_thread vs h1 == vget_model (v_thread vs h0) s v
+          )
+  = let ro = VCache.vcache_get_record vs.st s in
+    match ro with
     | None ->
-      fail vs "VGet: Empty slot"
-    | Some r' -> sladmit ()
-    // AF: Need to relate the two datatypes better, to ensure that the condition
-    // below is equivalent to stored_key (v_st vs.st h) s <> (data_key_v k)
-    //   if r'.T.record_key <> k then (fail vs "VGet: Key mismatch")
-    //   else begin
-    //   match r'.T.record_value with
-    //     | T.V_mval _ -> fail vs "VGet: Expected a data value"
-    //     | T.V_dval dv ->
-    //       if dv <> v then fail vs "VGet: Value mismatch"
-    //       else (noop (); sladmit())
-    //   end
-    //   // let k' = S.VStoreE?.k r' in
-    //   // let v' = S.VStoreE?.v r' in
-    //   // if key_v k <> k' then fail vs "VGet: Key mismatch"
-    //   // else if R.to_data_value v' <> value_v v then fail vs "VGet: Value mismatch"
-    //   // // AF: Usual problem of Steel vs SteelF difference in branches
-    //   // else (noop (); ())
-
-
-(* An implementation of Veritas.Intermediate.Verify.vput *)
-let vput (#vcfg:_) (s:slot_t vcfg) (k:data_key_t) (v:data_value_t) (vs:thread_state_t vcfg)
-  : Steel unit
-             (thread_state_inv vs)
-             (fun _ -> thread_state_inv vs)
-             (requires fun h0 ->
-               V.Valid? (v_thread vs h0))
-             (ensures fun h0 _ h1 ->
-               V.Valid? (v_thread vs h0)
-//               v_thread vs h1 == V.vput (U32.v s) (key_v k) (value_v v) (v_thread vs h0)
-               )
-  = // AF: Still unclear why this is needed
-    let h = get () in
-    assert (V.Valid? (v_thread vs h));
-
-    let r0 = vstore_get_record vs.st s in
-    match r0 with
-    | None -> fail vs "VPut: Empty slot"
+      fail vs "Slot not found"
     | Some r' ->
-      if r'.T.record_key <> k then fail vs "VPut: Key mismatch"
-      else (vstore_update_record vs.st s v; ())
+      if v = r'.T.record_value
+      // AF: Usual problem of Steel vs SteelF difference between the two branches
+      then (noop (); ())
+      else fail vs "Failed: inconsistent key or value in Get"
+
+(* verifier write operation *)
+let vput (s:U32.t) (v:T.value) (vs: thread_state_t)
+  : Steel unit
+    (thread_state_inv vs)
+    (fun _ -> thread_state_inv vs)
+    (requires fun h -> U32.v s < length (v_thread vs h).model_store)
+    (ensures fun h0 _ h1 ->
+      U32.v s < length (v_thread vs h0).model_store /\
+      v_thread vs h1 == vput_model (v_thread vs h0) s v)
+  = let ro = VCache.vcache_get_record vs.st s in
+    match ro with
+    | None ->
+      fail vs "Slot not found"
+
+    | Some r ->
+      vcache_update_record vs.st s ({ r with T.record_value = v });
+      ()
