steel/Veritas.Steel.VCache.fsti
@@ -1,0 +1,54 @@
+module Veritas.Steel.VCache
+
+open Steel.Memory
+open Steel.Effect
+open Steel.Effect.Atomic
+open Steel.FractionalPermission
+open FStar.Ghost
+module U32 = FStar.UInt32
+open Steel.Array
+
+module T = Veritas.Formats.Types
+open Veritas.Steel.VerifierModel
+
+let vstore : Type0 = Steel.Array.array (option T.record)
+unfold
+let is_vstore (st:vstore) = varray st
+
+val vcache_create (n:U32.t)
+  : Steel vstore
+           emp
+           (fun v -> is_vstore v)
+           (requires fun _ -> True)
+           (ensures fun _ v h1 -> asel v h1 == Seq.create (U32.v n) None)
+
+let slot_id = U32.t
+
+val vcache_get_record (vst:vstore) (s:slot_id)
+  : Steel (option T.record)
+          (is_vstore vst)
+          (fun _ -> is_vstore vst)
+          (requires fun h -> U32.v s < length (asel vst h))
+          (ensures fun h0 res h1 ->
+             U32.v s < length (asel vst h0) /\
+             asel vst h0 == asel vst h1 /\
+             res == Seq.index (asel vst h1) (U32.v s))
+
+val vcache_set (st:vstore) (s:slot_id) (r:option T.record)
+  : Steel unit
+      (is_vstore st)
+      (fun _ -> is_vstore st)
+      (requires fun h -> U32.v s < length (asel st h))
+      (ensures fun h0 _ h1 ->
+        U32.v s < length (asel st h0) /\
+        asel st h1 == Seq.upd (asel st h0) (U32.v s) r)
+
+let vcache_update_record (st:vstore) (s:slot_id) (r:T.record)
+  : Steel unit
+      (is_vstore st)
+      (fun _ -> is_vstore st)
+      (requires fun h -> U32.v s < length (asel st h))
+      (ensures fun h0 _ h1 ->
+        U32.v s < length (asel st h0) /\
+        asel st h1 == Seq.upd (asel st h0) (U32.v s) (Some r))
+  = vcache_set st s (Some r)
